src/ReactorModel/Objects/Reactor/ReactorType/Wellformed.lean
@@ -23,7 +23,7 @@ inductive Dependency [Indexable α] (rtr : α) : ID → ID → Prop
     (rcn₁.deps .out ∩ rcn₂.deps .in).Nonempty → Dependency rtr i₁ i₂
   | mutNest :
     (rtr[.rtr][i] = some rtr₁) → (nest rtr₁ j = some rtr₂) → (rcns rtr₁ iₘ = some m) → (m.Mutates) →
-    (iᵣ ∈ (rcns rtr₂).ids) → Dependency rtr iₘ iᵣ
+    (iᵣ ∈ rcns rtr₂) → Dependency rtr iₘ iᵣ
   | trans : 
     Dependency rtr i₁ i₂ → Dependency rtr i₂ i₃ → Dependency rtr i₁ i₃
 
@@ -53,7 +53,7 @@ theorem lower [c : LawfulCoe α β] (d : i₁ <[rtr] i₂) : i₁ <[(rtr : β)] 
     exact depOverlap (c.lower_obj?_some h₁) (c.lower_obj?_some h₂) ‹_›
   | mutNest h₁ h₂ h₃ _ h₄ => 
     exact mutNest (c.lower_obj?_some h₁) (c.lower_cpt?_eq_some .rtr h₂)
-          (c.lower_cpt?_eq_some .rcn h₃) ‹_› (c.lower_mem_cpt?_ids .rcn h₄) 
+          (c.lower_cpt?_eq_some .rcn h₃) ‹_› (c.lower_mem_cpt? .rcn h₄) 
   | trans _ _ d₁ d₂ => 
     exact trans d₁ d₂
 
@@ -76,7 +76,7 @@ theorem equiv (e : rtr₁ ≈ rtr₂) (d : j₁ <[rtr₂] j₂) : j₁ <[rtr₁]
     have ⟨_, h₁'⟩ := e.obj?_some_iff.mpr ⟨_, h₁⟩  
     have e := Equivalent.obj?_rtr_equiv e h₁' h₁
     have ⟨_, h₂'⟩ := cpt?_some_iff e (cpt := .rtr) |>.mpr ⟨_, h₂⟩
-    have h₄' := mem_cpt?_ids_iff (Equivalent.nest_equiv e h₂' h₂) (cpt := .rcn) |>.mpr h₄
+    have h₄' := mem_cpt?_iff (Equivalent.nest_equiv e h₂' h₂) (cpt := .rcn) |>.mpr h₄
     exact mutNest h₁' h₂' (rcns_eq e ▸ h₃) ‹_› h₄'
   | trans _ _ d₁ d₂ => 
     exact trans d₁ d₂
@@ -108,11 +108,11 @@ variable [ReactorType α] [ReactorType β] [LawfulCoe α β] {rtr : α} in secti
 -- `ValidDependency rtr .norm .in (.action i)` states that normal reactions can specify the action 
 -- identified by `i` as source.
 inductive ValidDependency (rtr : α) : Reaction.Kind → Kind → Reaction.Dependency → Prop
-  | act       : (i ∈ (acts rtr).ids) → ValidDependency rtr _ _ (.action i)
-  | prt       : (i ∈ (ports rtr dk).ids) → ValidDependency rtr _ dk (.port k i)
-  | nestedIn  : (nest rtr j = some con) → (i ∈ (ports con .in).ids) → 
+  | act       : (i ∈ acts rtr) → ValidDependency rtr _ _ (.action i)
+  | prt       : (i ∈ ports rtr dk) → ValidDependency rtr _ dk (.port k i)
+  | nestedIn  : (nest rtr j = some con) → (i ∈ ports con .in) → 
                 ValidDependency rtr _ .out (.port .in i)
-  | nestedOut : (nest rtr j = some con) → (i ∈ (ports con .out).ids) → 
+  | nestedOut : (nest rtr j = some con) → (i ∈ ports con .out) → 
                 ValidDependency rtr .norm .in (.port .in i)
 
 set_option hygiene false in
@@ -123,12 +123,12 @@ scoped macro "lift_nested_proof " name:ident : term => `(
     obtain ⟨_, _, h⟩ := h
     subst h
     exact $(Lean.mkIdentFrom name $ `ValidDependency ++ name.getId) 
-      (LawfulCoe.lift_cpt?_eq_some .rtr hc) (LawfulCoe.lift_mem_cpt?_ids (.prt _) hp)
+      (LawfulCoe.lift_cpt?_eq_some .rtr hc) (LawfulCoe.lift_mem_cpt? (.prt _) hp)
 )
 
 theorem ValidDependency.lift : (ValidDependency (rtr : β) rk dk d) → ValidDependency rtr rk dk d 
-  | act h           => act $ LawfulCoe.lift_mem_cpt?_ids .act h
-  | prt h           => prt $ LawfulCoe.lift_mem_cpt?_ids (.prt _) h
+  | act h           => act $ LawfulCoe.lift_mem_cpt? .act h
+  | prt h           => prt $ LawfulCoe.lift_mem_cpt? (.prt _) h
   | nestedIn hc hp  => (lift_nested_proof nestedIn) hc hp
   | nestedOut hc hp => (lift_nested_proof nestedOut) hc hp
     
@@ -143,23 +143,23 @@ scoped macro "equiv_nested_proof " name:ident : term => `(
     have ⟨_, hc'⟩ := Equivalent.cpt?_some_iff e (cpt := .rtr) |>.mp ⟨_, hc⟩ 
     have e := Equivalent.nest_equiv e hc hc'
     $(Lean.mkIdentFrom name $ `ValidDependency ++ name.getId) hc' 
-    (Equivalent.mem_cpt?_ids_iff e (cpt := .prt _) |>.mp hp)
+    (Equivalent.mem_cpt?_iff e (cpt := .prt _) |>.mp hp)
 )
 
 open Equivalent in
 theorem ValidDependency.equiv 
     (e : rtr₁ ≈ rtr₂) (h₁ : rtr₁[.rtr][j] = some con₁) (h₂ : rtr₂[.rtr][j] = some con₂) : 
     (ValidDependency con₁ rk dk d) → ValidDependency con₂ rk dk d
-  | act h           => act $ mem_cpt?_ids_iff (obj?_rtr_equiv e h₁ h₂) (cpt := .act) |>.mp h
-  | prt h           => prt $ mem_cpt?_ids_iff (obj?_rtr_equiv e h₁ h₂) (cpt := .prt _) |>.mp h
+  | act h           => act $ mem_cpt?_iff (obj?_rtr_equiv e h₁ h₂) (cpt := .act) |>.mp h
+  | prt h           => prt $ mem_cpt?_iff (obj?_rtr_equiv e h₁ h₂) (cpt := .prt _) |>.mp h
   | nestedIn hc hp  => (equiv_nested_proof nestedIn) hc hp
   | nestedOut hc hp => (equiv_nested_proof nestedOut) hc hp
 
 -- TODO: Refactor the `prio` conditions into one.
 structure _root_.ReactorType.Wellformed (rtr : α) : Prop where
   uniqueInputs : (rtr[.rcn][i₁] = some rcn₁) → (rtr[.rcn][i₂] = some rcn₂) → (i₁ ≠ i₂) → 
-                 (i ∈ rtr[.prt .in].ids) → (.port .in i ∈ rcn₁.deps .out) → 
-                 (.port .in i ∉ rcn₂.deps .out)  
+                 (i ∈ rtr[.prt .in]) → (.port .in i ∈ rcn₁.deps .out) → 
+                (.port .in i ∉ rcn₂.deps .out)  
   overlapPrio  : (rtr[.rtr][i] = some con) → (rcns con i₁ = some rcn₁) → (rcns con i₂ = some rcn₂) → 
                  (i₁ ≠ i₂) → (rcn₁.deps .out ∩ rcn₂.deps .out).Nonempty → 
                  (rcn₁.prio < rcn₂.prio ∨ rcn₂.prio < rcn₁.prio)
@@ -187,7 +187,7 @@ theorem nested (wf : Wellformed rtr₁) (h : nest rtr₁ i = some rtr₂) : Well
   validDeps               := wf_nested_proof validDeps
   acyclicDeps             := wf.acyclicDeps.nested h
   uniqueInputs h₁ h₂ _ h₄ := 
-    wf.uniqueInputs (obj?_nested h h₁) (obj?_nested h h₂) ‹_› (obj?_mem_ids_nested h h₄)
+    wf.uniqueInputs (obj?_nested h h₁) (obj?_nested h h₂) ‹_› (obj?_mem_nested h h₄)
 
 set_option hygiene false in 
 scoped macro "lift_prio_proof " name:ident : term => `(
@@ -204,7 +204,7 @@ theorem lift [c : LawfulCoe α β] (wf : Wellformed (rtr : β)) : Wellformed rtr
   validDeps h₁ h₂ h₃ := 
     wf.validDeps (c.lower_obj?_some h₁) (c.lower_cpt?_eq_some .rcn h₂) h₃ |>.lift
   uniqueInputs h₁ h₂ _ h₄ := 
-    wf.uniqueInputs (c.lower_obj?_some h₁) (c.lower_obj?_some h₂) ‹_› (c.lower_mem_obj?_ids h₄)
+    wf.uniqueInputs (c.lower_obj?_some h₁) (c.lower_obj?_some h₂) ‹_› (c.lower_mem_obj? h₄)
 
 set_option hygiene false in
 scoped macro "equiv_prio_proof " name:ident rtr₁:ident rtr₂:ident : term => `(
@@ -226,7 +226,7 @@ theorem equiv (e : rtr₁ ≈ rtr₂) (wf : Wellformed rtr₁) : Wellformed rtr�
     have h₂' := Equivalent.rcns_eq e ▸ h₂
     wf.validDeps h₁' h₂' h₃ |>.equiv ‹_› h₁' h₁
   uniqueInputs h₁ h₂ _ h₃ := 
-    have h₃' := Equivalent.mem_obj?_ids_iff e |>.mpr h₃
+    have h₃' := Equivalent.mem_iff e |>.mpr h₃
     wf.uniqueInputs (e.obj?_rcn_eq.symm ▸ h₁) (e.obj?_rcn_eq.symm ▸ h₂) ‹_› h₃'
 
 end Wellformed
